fix surface globals

Intermediate/Global.lean
@@ -1,14 +1,14 @@
 
 import Surface.Global
 import Core.Global
-
+import Core.Ty
 
 import Lilac
 open Lilac
 
 namespace Intermediate
 
-/-- Staged Global that contains pre-elaaborated terms, but compiled types and kinds -/
+/-- Staged Global that contains Surface level terms, but compiled types and kinds -/
 inductive Global : Type where
 | data : (n : Nat) -> String -> Core.Kind -> Vec (String × Core.SpineTy) n -> Global
 | defn : String -> Core.Ty -> Surface.Term -> Global
@@ -19,6 +19,20 @@ inductive Global : Type where
 | octor  : String -> Core.SpineTy -> Global
 | inst : {m : Nat} -> String -> Core.Pattern m -> Surface.Term -> Global
 
+
+def Global.repr (_ : Nat) : (a : Global) -> Std.Format
+| .data _ s K ctors =>
+  ".data " ++ s ++ " : " ++ Core.Kind.repr max_prec K  ++ " where " ++ Std.Format.line
+     ++ Std.Format.nest 4 (ctors.reprPrec 0)
+| .odata n K => ".odata " ++ n ++ " " ++ K.repr max_prec
+| .openm n ty => ".openm " ++ n ++ " : " ++ Core.SpineTy.repr ty
+| .defn n T t => ".defn " ++ n ++ " " ++ T.repr max_prec ++ Std.Format.line ++ t.repr max_prec
+| .inst n p t => ".inst " ++ n ++ " " ++ p.repr ++ " => " ++ t.repr max_prec
+| .octor n ty => ".octor " ++ n ++ " " ++ Core.SpineTy.repr ty
+
+@[simp]
+instance instRepr_Global : Repr Global where
+  reprPrec a p := Global.repr p a
 
 @[simp]
 abbrev GlobalEnv := List Global
@@ -31,7 +45,7 @@ inductive Entry : Type where
 | defn : String -> Core.Ty -> Surface.Term -> Entry
 | octor : String -> Core.SpineTy -> Entry
 
-def lookup (x : String) : List Global -> Option Entry := sorry
+def lookup (x : String) : GlobalEnv -> Option Entry := sorry
 
 inductive DataConst where
 | opn
