Surface/Global.lean
@@ -12,12 +12,12 @@ namespace Surface
 inductive Global where
 | data : {n : Nat} -> String -> Kind -> Vec (String × SpineTy) n -> Global
 | defn : String -> Ty -> Term -> Global
-| classDecl : {mc kc fc sc : Nat} ->
-  String -> Vec Kind kc ->
-  Vec (String × Ty) sc ->
-  Vec (String × Fin kc × Fin kc) fc ->
-  Vec (String × SpineTy) mc -> Global
-| instDecl : {mc : Nat} -> String -> SpineTy -> Vec (String × Term) mc -> Global
+| classDecl : {kc : Nat} ->
+  String -> Vec Kind kc -> -- TODO Change Vec to List for SC and determiners of FDs and methods
+  List (String × String × List (Fin kc)) ->
+  List (String × (n : Nat) × Vec (Fin kc) (n + 1) × Fin kc) ->
+  List (String × SpineTy) -> Global
+| instDecl : String -> SpineTy -> List (String × Term) -> Global  -- what to do with instance constraints and ty params?
 
 
 def Global.repr (_ : Nat) : (a : Global) -> Std.Format
@@ -29,10 +29,10 @@ def Global.repr (_ : Nat) : (a : Global) -> Std.Format
 | classDecl s Ks scs fds methods =>
   ".class " ++ s ++ " : " ++ Ks.repr max_prec ++ "|"  ++ scs.repr max_prec
     ++ "|" ++ fds.repr max_prec ++ (Std.Format.text " where ")
-    ++ Std.Format.line ++ (methods.reprPrec 0)
+    ++ Std.Format.line ++ (methods.repr max_prec)
 | instDecl i_name spTy methods =>
   (Std.Format.text ".inst ") ++ i_name ++ " : " ++ "⟨" ++ spTy.repr max_prec ++ "⟩"
-    ++ Std.Format.line ++ Std.Format.nest 4 (methods.reprPrec max_prec)
+    ++ Std.Format.line ++ Std.Format.nest 4 (methods.repr max_prec)
 
 @[simp]
 instance instRepr_Global : Repr (Global) where
@@ -47,7 +47,7 @@ inductive Entry : Type where
 | defn : String -> Ty -> Term -> Entry
 | odata : {n : Nat} -> String -> Vec Kind n -> Entry
 | octor : String -> SpineTy -> Entry
-| openm : String -> Nat -> SpineTy -> Entry
+| openm : String -> SpineTy -> Entry
 
 def Entry.is_data : Entry -> Bool
 | data _ _ _ => true
@@ -62,7 +62,7 @@ def Entry.is_odata : Entry -> Bool
 | _ => false
 
 def Entry.is_openm : Entry -> Bool
-| openm _ _ _ => true
+| openm _ _ => true
 | _ => false
 
 def Entry.is_defn : Entry -> Bool
@@ -85,12 +85,18 @@ def lookup (x : String) : GlobalEnv -> Option (Entry)
   else ctors'.to.foldl (init := lookup x tl) Option.or
 | .cons (.defn y a b) tl =>
   if x == y then return .defn y a b else lookup x tl
-| .cons (.classDecl (mc := n) y Ks _ _ ms) tl =>
-  let ms' : Fun.Vec (Option (Entry)) n := λ i =>
-    let (z, A) := ms.to i
-    if x == z then return .openm z i A else none
+| .cons (.classDecl (kc := kc) y Ks scs fds ms) tl =>
+  let ms_mb : Option (String × SpineTy) := ms.find? (λ (mn, _) => x == mn)
+  let ms := ms_mb.map (λ (x, mn) => .openm x mn)
+  let scs_mb : Option (String × String × List (Fin kc)) := scs.find? (λ (sc, _, _) => x == sc)
+  let scs := scs_mb.map (λ (scn, cls, tys) => .openm scn ⟨kc, Ks, 0, #(), 1, #((gt`#y).mkApps_nats (List.range kc)), (gt`#cls).mkApps_nats tys⟩ )
+  -- let fds_mb : Option (String × (n : Nat) × Vec (Fin kc) (n + 1) × Fin kc) := fds.find? (λ ⟨fdn, _, _, _⟩ => x == fdn)
+  -- let fds := fds_mb.map (λ ⟨fdn, n, dns, dt⟩ => Entry.openm fdn ⟨kc, Ks, 0, #(), 2, #(sorry, sorry), t`#0 ⟩)
   if x == y then return .odata y Ks
-  else ms'.to.foldl (init := lookup x tl) Option.or
+  else if ms.isSome then ms
+  else if scs.isSome then scs
+  -- else if fds.isSome then fds
+  else lookup x tl
 | .cons (.instDecl s spTy _) tl =>
   if x == s then return .octor s spTy
   else lookup x tl
@@ -98,11 +104,11 @@ def lookup (x : String) : GlobalEnv -> Option (Entry)
 def lookup_kind (G : GlobalEnv) (x : String) : Option Kind := lookup x G |> Option.map Entry.kind |> Option.get!
 
 
-def is_ctor (G : GlobalEnv) x := lookup x G |> Option.map Entry.is_ctor |> Option.get!
-def is_data (G : GlobalEnv) x := lookup x G |> Option.map Entry.is_data |> Option.get!
-def is_opent (G : GlobalEnv) x := lookup x G |> Option.map Entry.is_odata |> Option.get!
-def is_openm (G : GlobalEnv) x := lookup x G |> Option.map Entry.is_openm |> Option.get!
-def is_defn (G : GlobalEnv) x := lookup x G |> Option.map Entry.is_defn |> Option.get!
+-- def is_ctor (G : GlobalEnv) x := lookup x G |> Option.map Entry.is_ctor |> Option.get!
+-- def is_data (G : GlobalEnv) x := lookup x G |> Option.map Entry.is_data |> Option.get!
+-- def is_opent (G : GlobalEnv) x := lookup x G |> Option.map Entry.is_odata |> Option.get!
+-- def is_openm (G : GlobalEnv) x := lookup x G |> Option.map Entry.is_openm |> Option.get!
+-- def is_defn (G : GlobalEnv) x := lookup x G |> Option.map Entry.is_defn |> Option.get!
 
 def ctor_idx (x : String) (G : GlobalEnv) : Option Nat := do
   let t <- lookup x G
@@ -116,6 +122,6 @@ def Entry.name : Entry -> String
 | .defn n _ _
 | .odata n _
 | .octor n _
-| .openm n _ _ => n
+| .openm n _ => n
 
 end Surface
