Intermediate/Typing.lean
@@ -18,7 +18,4 @@ inductive VecTyping (J : A -> B -> Prop) : Vec A m -> Vec B m -> Prop
 def Query (G : List Global) (c : DataConst) (qs : Vec String m) (Ts : Vec Core.Ty m) : Prop :=
   VecTyping (lookup_ctor? G c · ·) qs Ts
 
-def Query.Match (qs : Vec String m) (ps : Core.Pattern m) : Prop :=
-  VecTyping (λ q p => ∃ na As nb, p = ⟨q, na, As, nb⟩) qs ps
-
 end Intermediate
